proof/refine/X64/ArchCSpace_I.thy
@@ -4,12 +4,10 @@
  * SPDX-License-Identifier: GPL-2.0-only
  *)
 
-(*
-   CSpace invariants
-*)
+(* CSpace invariants - architecture-specific *)
 
-theory CSpace_I
-imports ArchArchAcc_R
+theory ArchCSpace_I
+imports CSpace_I
 begin
 
 context begin interpretation Arch . (*FIXME: arch-split*)
@@ -23,25 +21,37 @@ lemma capUntypedPtr_simps [simp]:
   "capUntypedPtr (UntypedCap d r n f) = r"
   "capUntypedPtr (CNodeCap r n g n2) = r"
   "capUntypedPtr (ReplyCap r m a) = r"
-  "Arch.capUntypedPtr (ARM_H.ASIDPoolCap r asid) = r"
-  "Arch.capUntypedPtr (ARM_H.PageCap d r rghts sz mapdata) = r"
-  "Arch.capUntypedPtr (ARM_H.PageTableCap r mapdata2) = r"
-  "Arch.capUntypedPtr (ARM_H.PageDirectoryCap r mapdata3) = r"
+  "Arch.capUntypedPtr (X64_H.ASIDPoolCap r asid) = r"
+  "Arch.capUntypedPtr (X64_H.PageCap r rghts mt sz d mapdata) = r"
+  "Arch.capUntypedPtr (X64_H.PageTableCap r mapdata2) = r"
+  "Arch.capUntypedPtr (X64_H.PageDirectoryCap r mapdata3) = r"
+  "Arch.capUntypedPtr (X64_H.PDPointerTableCap r mapdata4) = r"
+  "Arch.capUntypedPtr (X64_H.PML4Cap r mapdata5) = r"
   by (auto simp: capUntypedPtr_def
-                 ARM_H.capUntypedPtr_def)
+                 X64_H.capUntypedPtr_def)
 
 lemma rights_mask_map_UNIV [simp]:
   "rights_mask_map UNIV = allRights"
   by (simp add: rights_mask_map_def allRights_def)
 
+declare insert_UNIV[simp]
+
 lemma maskCapRights_allRights [simp]:
   "maskCapRights allRights c = c"
   unfolding maskCapRights_def isCap_defs allRights_def
-            ARM_H.maskCapRights_def maskVMRights_def
+            X64_H.maskCapRights_def maskVMRights_def
   by (cases c) (simp_all add: Let_def split: arch_capability.split vmrights.split)
 
 lemma getCTE_inv [wp]: "\<lbrace>P\<rbrace> getCTE addr \<lbrace>\<lambda>rv. P\<rbrace>"
   by (simp add: getCTE_def) wp
+
+lemma getEndpoint_inv [wp]:
+  "\<lbrace>P\<rbrace> getEndpoint ptr \<lbrace>\<lambda>rv. P\<rbrace>"
+  by (simp add: getEndpoint_def getObject_inv loadObject_default_inv)
+
+lemma getNotification_inv [wp]:
+  "\<lbrace>P\<rbrace> getNotification ptr \<lbrace>\<lambda>rv. P\<rbrace>"
+  by (simp add: getNotification_def getObject_inv loadObject_default_inv)
 
 lemma getSlotCap_inv [wp]: "\<lbrace>P\<rbrace> getSlotCap addr \<lbrace>\<lambda>rv. P\<rbrace>"
   by (simp add: getSlotCap_def, wp)
@@ -273,6 +283,39 @@ lemma no_0_update:
   shows "no_0 (m(p \<mapsto> cte))"
   using no0 pnz unfolding no_0_def by simp
 
+lemma has_loop_update:
+  assumes lp: "m(p \<mapsto> cte) \<turnstile> c \<leadsto>\<^sup>+ c'"
+  and    cn0: "c' \<noteq> 0"
+  and  mnext: "mdbNext (cteMDBNode cte) = 0"
+  and    mn0: "no_0 m"
+  and    pn0: "p \<noteq> 0"
+  shows "m \<turnstile> c \<leadsto>\<^sup>+ c'"
+  using lp cn0
+proof induct
+  case (base y)
+  have "m \<turnstile> c \<leadsto> y"
+  proof (rule mdb_next_update_other)
+    show "p \<noteq> c" using base
+      by (clarsimp intro: contrapos_nn simp: mdb_next_update mnext)
+  qed fact+
+
+  thus ?case ..
+next
+  case (step y z)
+
+  show ?case
+  proof
+    have "y \<noteq> 0" by (rule no_0_lhs [OF _  no_0_update]) fact+
+    thus "m \<turnstile> c \<leadsto>\<^sup>+ y" using step by simp
+  next
+    have "z \<noteq> 0" by fact+
+    hence "p \<noteq> y" using step.hyps mnext
+      by (clarsimp simp: mdb_next_update)
+    thus "m \<turnstile> y \<leadsto> z"
+      by (rule mdb_next_update_other [OF step.hyps(2)])
+  qed
+qed
+
 lemma mdb_rtrancl_update_other:
   assumes  upd: "m(p \<mapsto> cte) \<turnstile> x \<leadsto>\<^sup>* y"
   and   nopath: "\<not> m \<turnstile> x \<leadsto>\<^sup>* p"
@@ -282,9 +325,7 @@ proof (cases rule: next_rtrancl_tranclE)
   case eq thus ?thesis by simp
 next
   case trancl thus ?thesis
-    by (auto del: trancl_into_rtrancl
-             intro: trancl_into_rtrancl
-             elim: mdb_trancl_update_other [OF _ nopath])
+    by (auto intro: trancl_into_rtrancl elim: mdb_trancl_update_other [OF _ nopath])
 qed
 
 lemma mdb_trancl_other_update:
@@ -320,9 +361,7 @@ proof (cases rule: next_rtrancl_tranclE)
   case eq thus ?thesis by simp
 next
   case trancl thus ?thesis
-    by (auto del: trancl_into_rtrancl
-             intro: trancl_into_rtrancl
-             elim: mdb_trancl_other_update [OF _ nopath])
+    by (auto intro: trancl_into_rtrancl elim: mdb_trancl_other_update [OF _ nopath])
 qed
 
 lemma mdb_chain_0_update:
@@ -512,7 +551,7 @@ lemma isDomainCap [simp]:
 
 lemma isPhysicalCap[simp]:
   "isPhysicalCap cap = (capClass cap = PhysicalClass)"
-  by (simp add: isPhysicalCap_def ARM_H.isPhysicalCap_def
+  by (simp add: isPhysicalCap_def X64_H.isPhysicalCap_def
          split: capability.split arch_capability.split)
 
 (* FIXME instead of a definition and then a simp rule in the simp set, we should use fun *)
@@ -527,14 +566,18 @@ where
  | ReplyCap ref master g \<Rightarrow> ReplyCap ref True True
  | UntypedCap d ref n f \<Rightarrow> UntypedCap d ref n 0
  | ArchObjectCap acap \<Rightarrow> ArchObjectCap (case acap of
-      PageCap d ref rghts sz mapdata \<Rightarrow>
-         PageCap d ref VMReadWrite sz None
+      PageCap ref rghts mt sz d mapdata \<Rightarrow>
+         PageCap ref VMReadWrite VMNoMap sz d None
     | ASIDPoolCap pool asid \<Rightarrow>
          ASIDPoolCap pool 0
     | PageTableCap ptr data \<Rightarrow>
          PageTableCap ptr None
     | PageDirectoryCap ptr data \<Rightarrow>
          PageDirectoryCap ptr None
+    | PDPointerTableCap ptr data \<Rightarrow>
+         PDPointerTableCap ptr None
+    | PML4Cap ptr data \<Rightarrow>
+         PML4Cap ptr None
     | _ \<Rightarrow> acap)
  | _ \<Rightarrow> cap"
 
@@ -543,25 +586,30 @@ lemma capMasterCap_simps[simp]:
   "capMasterCap (NotificationCap ref bdg s r) = NotificationCap ref 0 True True"
   "capMasterCap (CNodeCap ref bits gd gs) = CNodeCap ref bits 0 0"
   "capMasterCap (ThreadCap ref) = ThreadCap ref"
-  "capMasterCap capability.NullCap = capability.NullCap"
-  "capMasterCap capability.DomainCap = capability.DomainCap"
-  "capMasterCap (capability.IRQHandlerCap irq) = capability.IRQHandlerCap irq"
-  "capMasterCap (capability.Zombie word zombie_type n) = capability.Zombie word zombie_type n"
-  "capMasterCap (capability.ArchObjectCap (arch_capability.ASIDPoolCap word1 word2)) =
-            capability.ArchObjectCap (arch_capability.ASIDPoolCap word1 0)"
-  "capMasterCap (capability.ArchObjectCap arch_capability.ASIDControlCap) =
-         capability.ArchObjectCap arch_capability.ASIDControlCap"
-  "capMasterCap (capability.ArchObjectCap (arch_capability.PageCap d word vmrights vmpage_size pdata)) =
-            capability.ArchObjectCap (arch_capability.PageCap d word VMReadWrite vmpage_size None)"
-  "capMasterCap (capability.ArchObjectCap (arch_capability.PageTableCap word ptdata)) =
-            capability.ArchObjectCap (arch_capability.PageTableCap word None)"
-  "capMasterCap (capability.ArchObjectCap (arch_capability.PageDirectoryCap word pddata)) =
-            capability.ArchObjectCap (arch_capability.PageDirectoryCap word None)"
-  "capMasterCap (capability.ArchObjectCap (arch_capability.SGISignalCap s_irq target)) =
-            capability.ArchObjectCap (arch_capability.SGISignalCap s_irq target)"
-  "capMasterCap (capability.UntypedCap d word n f) = capability.UntypedCap d word n 0"
-  "capMasterCap capability.IRQControlCap = capability.IRQControlCap"
-  "capMasterCap (capability.ReplyCap word m g) = capability.ReplyCap word True True"
+  "capMasterCap NullCap = NullCap"
+  "capMasterCap DomainCap = DomainCap"
+  "capMasterCap (IRQHandlerCap irq) = IRQHandlerCap irq"
+  "capMasterCap (Zombie word zombie_type n) = Zombie word zombie_type n"
+  "capMasterCap (ArchObjectCap (ASIDPoolCap word1 word2)) =
+            ArchObjectCap (ASIDPoolCap word1 0)"
+  "capMasterCap (ArchObjectCap ASIDControlCap) =
+            ArchObjectCap ASIDControlCap"
+  "capMasterCap (ArchObjectCap (PageCap word vmrights mt vmpage_size d pdata)) =
+            ArchObjectCap (PageCap word VMReadWrite VMNoMap vmpage_size d None)"
+  "capMasterCap (ArchObjectCap (PageTableCap word ptdata)) =
+            ArchObjectCap (PageTableCap word None)"
+  "capMasterCap (ArchObjectCap (PageDirectoryCap word pddata)) =
+            ArchObjectCap (PageDirectoryCap word None)"
+  "capMasterCap (ArchObjectCap (PDPointerTableCap word pdptdata)) =
+            ArchObjectCap (PDPointerTableCap word None)"
+  "capMasterCap (ArchObjectCap (PML4Cap word pml4data)) =
+            ArchObjectCap (PML4Cap word None)"
+  "capMasterCap (ArchObjectCap (IOPortCap ft lt)) =
+            ArchObjectCap (IOPortCap ft lt)"
+  "capMasterCap (ArchObjectCap IOPortControlCap) = ArchObjectCap IOPortControlCap"
+  "capMasterCap (UntypedCap d word n f) = UntypedCap d word n 0"
+  "capMasterCap IRQControlCap = IRQControlCap"
+  "capMasterCap (ReplyCap word m g) = ReplyCap word True True"
   by (simp_all add: capMasterCap_def)
 
 lemma capMasterCap_eqDs1:
@@ -589,9 +637,9 @@ lemma capMasterCap_eqDs1:
      \<Longrightarrow> \<exists>f. cap = UntypedCap d ref bits f"
   "capMasterCap cap = ReplyCap ref master g
      \<Longrightarrow> master \<and> g \<and> (\<exists>master g. cap = ReplyCap ref master g)"
-  "capMasterCap cap = ArchObjectCap (PageCap d ref rghts sz mapdata)
-     \<Longrightarrow> rghts = VMReadWrite \<and> mapdata = None
-          \<and> (\<exists>rghts mapdata. cap = ArchObjectCap (PageCap d ref rghts sz mapdata))"
+  "capMasterCap cap = ArchObjectCap (PageCap ref rghts mt sz d mapdata)
+     \<Longrightarrow> rghts = VMReadWrite \<and> mapdata = None \<and> mt = VMNoMap
+          \<and> (\<exists>rghts mapdata mt. cap = ArchObjectCap (PageCap ref rghts mt sz d mapdata))"
   "capMasterCap cap = ArchObjectCap ASIDControlCap
      \<Longrightarrow> cap = ArchObjectCap ASIDControlCap"
   "capMasterCap cap = ArchObjectCap (ASIDPoolCap pool asid)
@@ -600,13 +648,21 @@ lemma capMasterCap_eqDs1:
      \<Longrightarrow> data = None \<and> (\<exists>data. cap = ArchObjectCap (PageTableCap ptr data))"
   "capMasterCap cap = ArchObjectCap (PageDirectoryCap ptr data2)
      \<Longrightarrow> data2 = None \<and> (\<exists>data2. cap = ArchObjectCap (PageDirectoryCap ptr data2))"
+  "capMasterCap cap = ArchObjectCap (PDPointerTableCap ptr data3)
+     \<Longrightarrow> data3 = None \<and> (\<exists>data3. cap = ArchObjectCap (PDPointerTableCap ptr data3))"
+  "capMasterCap cap = ArchObjectCap (PML4Cap ptr data4)
+     \<Longrightarrow> data4 = None \<and> (\<exists>data4. cap = ArchObjectCap (PML4Cap ptr data4))"
+  "capMasterCap cap = ArchObjectCap (IOPortCap first_port last_port)
+     \<Longrightarrow> cap = ArchObjectCap (IOPortCap first_port last_port)"
+  "capMasterCap cap = ArchObjectCap IOPortControlCap
+     \<Longrightarrow> cap = ArchObjectCap IOPortControlCap"
   by (clarsimp simp: capMasterCap_def
               split: capability.split_asm arch_capability.split_asm)+
 
 lemmas capMasterCap_eqDs[dest!] = capMasterCap_eqDs1 capMasterCap_eqDs1 [OF sym]
 
 definition
-  capBadge :: "capability \<Rightarrow> word32 option"
+  capBadge :: "capability \<Rightarrow> machine_word option"
 where
  "capBadge cap \<equiv> if isEndpointCap cap then Some (capEPBadge cap)
                  else if isNotificationCap cap then Some (capNtfnBadge cap)
@@ -655,22 +711,22 @@ lemma isCap_Master:
   "isNullCap (capMasterCap cap) = isNullCap cap"
   "isDomainCap (capMasterCap cap) = isDomainCap cap"
   "isArchPageCap (capMasterCap cap) = isArchPageCap cap"
-  "isArchObjectCap cap \<Longrightarrow> isSGISignalCap (capCap (capMasterCap cap)) = isSGISignalCap (capCap cap)"
-  "isArchSGISignalCap (capMasterCap cap) = isArchSGISignalCap cap"
-  by (auto simp: isCap_simps capMasterCap_def
-           split: capability.split arch_capability.split)
+  "isArchIOPortCap (capMasterCap cap) = isArchIOPortCap cap"
+  "isIOPortControlCap' (capMasterCap cap) = isIOPortControlCap' cap"
+  by (simp add: isCap_simps capMasterCap_def
+         split: capability.split arch_capability.split)+
 
 lemma capUntypedSize_capBits:
   "capClass cap = PhysicalClass \<Longrightarrow> capUntypedSize cap = 2 ^ (capBits cap)"
-  apply (simp add: capUntypedSize_def objBits_simps
-                   ARM_H.capUntypedSize_def
-                   pteBits_def pdeBits_def
-                   ptBits_def pdBits_def
-                   shiftl_eq_mult bit_simps'
+  apply (simp add: capUntypedSize_def objBits_simps'
+                   X64_H.capUntypedSize_def bit_simps
             split: capability.splits arch_capability.splits
                    zombie_type.splits)
   apply fastforce
   done
+
+(* unused in this architecture *)
+declare isIRQControlCapDescendant_def[simp]
 
 lemma sameRegionAs_def2:
  "sameRegionAs cap cap' = (\<lambda>cap cap'.
@@ -682,7 +738,7 @@ lemma sameRegionAs_def2:
       \<or> (capRange cap' \<noteq> {} \<and> capRange cap' \<subseteq> capRange cap
                  \<and> (isUntypedCap cap \<or> (isArchPageCap cap \<and> isArchPageCap cap')))
       \<or> (isIRQControlCap cap \<and> isIRQHandlerCap cap')
-      \<or> (isIRQControlCap cap \<and> isArchSGISignalCap cap'))
+      \<or> (isIOPortControlCap' cap \<and> isArchIOPortCap cap'))
            (capMasterCap cap) (capMasterCap cap')"
   apply (cases "isUntypedCap cap")
    apply (clarsimp simp: sameRegionAs_def Let_def
@@ -693,38 +749,37 @@ lemma sameRegionAs_def2:
    apply (intro impI iffI)
     apply (clarsimp del: subsetI intro!: range_subsetI)
    apply clarsimp
-   apply (simp add: range_subset_eq2)
   apply (simp cong: conj_cong)
   apply (simp     add: capMasterCap_def sameRegionAs_def isArchPageCap_def
                 split: capability.split
             split del: if_split cong: if_cong)
-  apply (simp    add: ARM_H.sameRegionAs_def isCap_simps
+  apply (simp    add: X64_H.sameRegionAs_def isCap_simps
                split: arch_capability.split
            split del: if_split cong: if_cong)
-  apply (clarsimp simp: capRange_def Let_def)
+  apply (clarsimp simp: capRange_def Let_def isCap_simps)
   apply (simp add: range_subset_eq2 cong: conj_cong)
-  by (simp add: conj_comms isIRQControlCapDescendant_def)
+  apply (simp add: conj_comms)
+  apply fastforce
+  done
 
 lemma sameObjectAs_def2:
  "sameObjectAs cap cap' = (\<lambda>cap cap'.
      (cap = cap'
-          \<and> (\<not> isNullCap cap \<and> \<not> isZombie cap
-              \<and> \<not> isUntypedCap cap)
-          \<and> (\<not> isNullCap cap' \<and> \<not> isZombie cap'
-              \<and> \<not> isUntypedCap cap')
+          \<and> (\<not> isNullCap cap \<and> \<not> isZombie cap \<and> \<not> isUntypedCap cap)
+          \<and> (\<not> isNullCap cap' \<and> \<not> isZombie cap' \<and> \<not> isUntypedCap cap')
           \<and> (isArchPageCap cap \<longrightarrow> capRange cap \<noteq> {})
           \<and> (isArchPageCap cap' \<longrightarrow> capRange cap' \<noteq> {})
-          \<and> \<not>isIRQControlCap cap
-          \<and> \<not>isArchSGISignalCap cap))
-           (capMasterCap cap) (capMasterCap cap')"
+          \<and> \<not>isIRQControlCap cap))
+        (capMasterCap cap) (capMasterCap cap')"
   apply (simp add: sameObjectAs_def sameRegionAs_def2
                    isCap_simps capMasterCap_def
             split: capability.split)
-  apply (clarsimp simp: ARM_H.sameObjectAs_def isCap_simps
+  apply (clarsimp simp: X64_H.sameObjectAs_def isCap_simps
                  split: arch_capability.split cong: if_cong)
-  apply (clarsimp simp: ARM_H.sameRegionAs_def isCap_simps
-             split del: if_split cong: if_cong)
-  apply (simp add: capRange_def)
+  apply (clarsimp simp: X64_H.sameRegionAs_def isCap_simps
+                  split del: if_split cong: if_cong)
+  apply (simp add: capRange_def isCap_simps
+              split del: if_split)
   by fastforce
 
 lemmas sameRegionAs_def3 =
@@ -736,14 +791,14 @@ lemmas sameObjectAs_def3 =
 lemma sameRegionAsE:
   "\<lbrakk> sameRegionAs cap cap';
      \<lbrakk> capMasterCap cap = capMasterCap cap'; \<not> isNullCap cap; \<not> isZombie cap;
-         \<not> isUntypedCap cap; \<not> isArchPageCap cap \<rbrakk> \<Longrightarrow> R;
+         \<not> isUntypedCap cap; \<not> isArchPageCap cap\<rbrakk> \<Longrightarrow> R;
      \<lbrakk> capRange cap' \<noteq> {}; capRange cap' \<subseteq> capRange cap; isUntypedCap cap \<rbrakk> \<Longrightarrow> R;
      \<lbrakk> capRange cap' \<noteq> {}; capRange cap' \<subseteq> capRange cap; isArchPageCap cap;
           isArchPageCap cap' \<rbrakk> \<Longrightarrow> R;
      \<lbrakk> isIRQControlCap cap; isIRQHandlerCap cap' \<rbrakk> \<Longrightarrow> R;
-     \<lbrakk> isIRQControlCap cap; isArchSGISignalCap cap' \<rbrakk> \<Longrightarrow> R
+     \<lbrakk> isIOPortControlCap' cap; isArchIOPortCap cap' \<rbrakk> \<Longrightarrow> R
       \<rbrakk> \<Longrightarrow> R"
-  by  (simp add: sameRegionAs_def3, fastforce simp: isCap_Master)
+   by  (simp add: sameRegionAs_def3, fastforce)
 
 lemma sameObjectAsE:
   "\<lbrakk> sameObjectAs cap cap';
@@ -754,15 +809,21 @@ lemma sameObjectAsE:
 
 lemma sameObjectAs_sameRegionAs:
   "sameObjectAs cap cap' \<Longrightarrow> sameRegionAs cap cap'"
-  by (clarsimp simp add: sameObjectAs_def2 sameRegionAs_def2)
+  by (clarsimp simp add: sameObjectAs_def2 sameRegionAs_def2 isCap_simps)
 
 lemma sameObjectAs_sym:
   "sameObjectAs c d = sameObjectAs d c"
-  by (auto simp: sameObjectAs_def2)
+  by (auto simp add: sameObjectAs_def2 eq_commute conj_comms)
 
 lemma untypedRange_Master:
   "untypedRange (capMasterCap cap) = untypedRange cap"
   by (simp add: capMasterCap_def split: capability.split)
+
+lemma sameObject_capRange:
+  "sameObjectAs cap cap' \<Longrightarrow> capRange cap' = capRange cap"
+  apply (rule master_eqI, rule capRange_Master)
+  apply (clarsimp simp: sameObjectAs_def2)
+  done
 
 lemma sameRegionAs_Null [simp]:
   "sameRegionAs c NullCap = False"
@@ -787,7 +848,7 @@ lemma capUntypedSize_simps [simp]:
   "capUntypedSize (ReplyCap r m a) = 1 << objBits (undefined :: tcb)"
   "capUntypedSize IRQControlCap = 1"
   "capUntypedSize (IRQHandlerCap irq) = 1"
-  by (auto simp add: capUntypedSize_def isCap_simps objBits_simps
+  by (auto simp add: capUntypedSize_def isCap_simps objBits_simps'
               split: zombie_type.splits)
 
 lemma sameRegionAs_classes:
@@ -796,9 +857,7 @@ lemma sameRegionAs_classes:
       apply (rule master_eqI, rule capClass_Master)
       apply simp
      apply (simp add: capRange_def split: if_split_asm)
-    apply (clarsimp simp: isCap_simps)
-   apply (clarsimp simp: isCap_simps)
-  apply (clarsimp simp: isCap_simps)
+    apply (clarsimp simp: isCap_simps)+
   done
 
 lemma capAligned_capUntypedPtr:
@@ -822,15 +881,10 @@ lemma sameRegionAs_capRange_Int:
   apply (clarsimp simp: isCap_simps)
   done
 
-lemma capRange_empty_simps[simp]:
-  "capRange IRQControlCap = {}"
-  "capRange (ArchObjectCap (SGISignalCap irq target)) = {}"
-  by (auto simp: capRange_def)
-
 lemma sameRegionAs_trans:
   "\<lbrakk> sameRegionAs a b; sameRegionAs b c \<rbrakk> \<Longrightarrow> sameRegionAs a c"
-  unfolding sameRegionAs_def2
-  by (elim conjE disjE, auto simp: isCap_simps)
+  apply (simp add: sameRegionAs_def2, elim conjE disjE, simp_all)
+                by (auto simp: isCap_simps capRange_def) (* long *)
 
 lemma capMasterCap_maskCapRights[simp]:
   "capMasterCap (maskCapRights msk cap)
@@ -839,7 +893,7 @@ lemma capMasterCap_maskCapRights[simp]:
          simp add: maskCapRights_def Let_def isCap_simps capMasterCap_def)
   apply (rename_tac arch_capability)
   apply (case_tac arch_capability;
-         simp add: ARM_H.maskCapRights_def Let_def isCap_simps)
+         simp add: X64_H.maskCapRights_def Let_def isCap_simps)
   done
 
 lemma capBadge_maskCapRights[simp]:
@@ -849,7 +903,7 @@ lemma capBadge_maskCapRights[simp]:
          simp add: maskCapRights_def Let_def isCap_simps capBadge_def)
   apply (rename_tac arch_capability)
   apply (case_tac arch_capability;
-         simp add: ARM_H.maskCapRights_def Let_def isCap_simps)
+         simp add: X64_H.maskCapRights_def Let_def isCap_simps)
   done
 
 lemma getObject_cte_det:
@@ -1152,7 +1206,7 @@ lemma cte_refs_capRange:
    \<comment> \<open>CNodeCap\<close>
    apply (clarsimp simp: objBits_simps capAligned_def shiftl_t2n' mask_def dest!: valid_capAligned)
    apply (rename_tac word1 nat1 word2 nat2 x)
-   apply (subgoal_tac "x * 2 ^ cteSizeBits < 2 ^ (cteSizeBits + nat1)")
+   apply (subgoal_tac "x * 2^cteSizeBits < 2 ^ (cteSizeBits + nat1)")
     apply (intro conjI)
      apply (erule(1) is_aligned_no_wrap')
     apply (simp add: add_diff_eq[symmetric])
@@ -1168,9 +1222,9 @@ lemma cte_refs_capRange:
    apply (simp only: power_add)
    apply (simp add: word_bits_def)
   \<comment> \<open>Zombie\<close>
-  apply (clarsimp simp: capAligned_def valid_cap'_def objBits_simps shiftl_t2n' mask_def)
-  apply (rename_tac word zombie_type nat x)
-  apply (subgoal_tac "x * 2^cteSizeBits < 2 ^ zBits zombie_type")
+  apply (rename_tac word zombie_type nat)
+  apply (clarsimp simp: capAligned_def valid_cap'_def objBits_simps shiftl_t2n' mask_def )
+  apply (subgoal_tac "xa * 2^cteSizeBits < 2 ^ zBits zombie_type")
    apply (intro conjI)
     apply (erule(1) is_aligned_no_wrap')
    apply (simp add: add_diff_eq[symmetric])
@@ -1369,7 +1423,8 @@ lemma
   untyped_inc: "untyped_inc' m" and
   class_links: "class_links m" and
   irq_control: "irq_control m"
-  using valid by (simp add: valid_mdb_ctes_def)+
+  using valid
+  by (simp_all add: valid_mdb_ctes_def)
 
 end (* of context vmdb *)
 
@@ -1646,7 +1701,7 @@ lemma untypedRange_not_emptyD: "untypedRange c' \<noteq> {} \<Longrightarrow> is
 lemma usableRange_subseteq:
   "\<lbrakk>capAligned c';isUntypedCap c'\<rbrakk> \<Longrightarrow> usableUntypedRange c' \<subseteq> untypedRange c'"
   apply (clarsimp simp: gen_isCap_simps capAligned_def shiftl_t2n' mask_def field_simps
-                  split: if_splits)
+                  split:if_splits)
   apply (erule order_trans[OF is_aligned_no_wrap'])
    apply (erule of_nat_power)
    apply (simp add:word_bits_def)+
@@ -1793,7 +1848,7 @@ lemma capBits_Master:
 
 lemma capUntyped_Master:
   "capUntypedPtr (capMasterCap cap) = capUntypedPtr cap"
-  by (clarsimp simp: capMasterCap_def split: capability.split arch_capability.split)
+  by (clarsimp simp: capMasterCap_def X64_H.capUntypedPtr_def split: capability.split arch_capability.split)
 
 lemma distinct_zombies_copyMasterE:
   "\<lbrakk> distinct_zombies m; m x = Some cte;
@@ -1910,7 +1965,8 @@ lemma valid_mdb_ctes_init:
      caps_no_overlap' m (capRange cap); s \<turnstile>' cap;
      valid_objs' s; m = ctes_of s; cap \<noteq> NullCap;
      fresh_virt_cap_class (capClass cap) (ctes_of s);
-     cap = capability.IRQControlCap \<longrightarrow> no_irq' (ctes_of s) \<rbrakk> \<Longrightarrow>
+     cap = capability.IRQControlCap \<longrightarrow> no_irq' (ctes_of s);
+     cap = capability.ArchObjectCap IOPortControlCap \<longrightarrow> no_ioport' (ctes_of s) \<rbrakk> \<Longrightarrow>
   valid_mdb_ctes (m (p \<mapsto> CTE cap initMDBNode))"
   apply (simp add: valid_mdb_ctes_def)
   apply (rule conjI, rule valid_dlist_init, simp+)
@@ -1959,13 +2015,14 @@ lemma setCTE_valid_mdb:
         s \<turnstile>' cap \<and> valid_objs' s \<and> cap \<noteq> NullCap \<and>
         caps_no_overlap' (ctes_of s) (capRange cap) \<and>
         fresh_virt_cap_class (capClass cap) (ctes_of s) \<and>
-        (cap = capability.IRQControlCap \<longrightarrow> no_irq' (ctes_of s))\<rbrace>
+        (cap = capability.IRQControlCap \<longrightarrow> no_irq' (ctes_of s)) \<and>
+        (cap = capability.ArchObjectCap IOPortControlCap \<longrightarrow> no_ioport' (ctes_of s))\<rbrace>
   setCTE ptr cte
   \<lbrace>\<lambda>r. valid_mdb'\<rbrace>"
   apply (simp add: valid_mdb'_def setCTE_def cte_def cte_wp_at_ctes_of)
   apply (wp ctes_of_setObject_cte)
   apply (clarsimp simp del: fun_upd_apply)
-  apply (erule(8) valid_mdb_ctes_init [OF _ _ _ _ _ _ refl])
+  apply (erule(9) valid_mdb_ctes_init [OF _ _ _ _ _ _ refl])
   done
 
 lemma setCTE_valid_objs'[wp]:
@@ -1974,7 +2031,7 @@ lemma setCTE_valid_objs'[wp]:
   unfolding setCTE_def
   apply (rule setObject_valid_objs')
    apply (clarsimp simp: prod_eq_iff lookupAround2_char1 updateObject_cte objBits_simps)
-   apply (clarsimp simp: prod_eq_iff lookupAround2_char1
+  apply (clarsimp simp: prod_eq_iff lookupAround2_char1
                          updateObject_cte in_monad typeError_def
                          valid_obj'_def valid_tcb'_def valid_cte'_def
                          tcb_cte_cases_def tcb_cte_cases_neqs
@@ -2014,6 +2071,8 @@ lemma getCTE_ctes_wp:
 lemma updateMDB_valid_objs'[wp]:
   "\<lbrace>valid_objs'\<rbrace> updateMDB m p \<lbrace>\<lambda>rv. valid_objs'\<rbrace>"
   apply (clarsimp simp add: updateMDB_def)
+apply (wp setCTE_valid_objs')
+
   apply (wp | simp)+
   done
 
@@ -2025,7 +2084,17 @@ lemma setCTE_no_0_obj' [wp]:
   "\<lbrace>no_0_obj'\<rbrace> setCTE p c \<lbrace>\<lambda>_. no_0_obj'\<rbrace>"
   by (simp add: setCTE_def) wp
 
+crunch setCTE
+  for pspace_canonical'[wp]: "pspace_canonical'"
+
+crunch setCTE
+  for pspace_in_kernel_mappings'[wp]: "pspace_in_kernel_mappings'"
+
 declare mresults_fail[simp]
+
+crunch get_object
+  for idle[wp]: "valid_idle"
+  (wp: crunch_wps simp: crunch_simps)
 
 end
 
